[WIP] After some tweaking, expand is properly defined.

theories/Rtree.v
@@ -2,6 +2,7 @@ Require Import List Program Arith Omega.
 
 (** ========== Common library ========== *)
 
+Arguments skipn [_] !n !l.
 Ltac inv H := inversion H; subst; clear H.
 
 (** === Indexed Forall === *)
@@ -110,24 +111,21 @@ Ltac gen_safe_proof :=
         generalize H as Hs
   end.
 
+(* FIXME No need for [proof_irrelevance]. *)
+Lemma lt_irrelevance {n m : nat} (p q : n < m): p = q.
+Proof.
+  apply proof_irrelevance.
+Qed.
+
+Ltac prove_lt_irrelevance := apply lt_irrelevance.
+Ltac unify_lt_proofs :=
+  repeat match goal with
+  | H1 : ?x < ?y, H2 : ?x < ?y |- _ =>
+      revert dependent H2; intros H2;
+      assert (H1 = H2) as <- by prove_lt_irrelevance
+  end.
+
 (* A few lemmas about [safe_nth] and standard list definitions. *)
-
-Lemma safe_nth_app2 {A : Type} (l1 l2 : list A) (n : nat) H1 H2 :
-  safe_nth (l1 ++ l2) (length l1 + n ; H1) = safe_nth l2 (n ; H2).
-Proof.
-  induction l1; simpl in *.
-  - f_equal. f_equal. 
-    (* We could do without [proof_irrelevance]. *) apply proof_irrelevance.
-  - erewrite <- IHl1. reflexivity.
-Qed.
-
-Lemma safe_nth_app2' {A : Type} (l1 l2 : list A) (n : nat) H1 H2 :
-  safe_nth (l1 ++ l2) (n + length l1 ; H1) = safe_nth l2 (n ; H2).
-Proof.
-  simpl in *. revert H1.
-  rewrite plus_comm; intros H1.
-  apply safe_nth_app2.
-Qed.
 
 Lemma safe_nth_app1 {A : Type} (l1 l2 : list A) (n : nat) H1 H2 :
   safe_nth (l1 ++ l2) (n ; H1) = safe_nth l1 (n ; H2).
@@ -139,6 +137,18 @@ Proof.
   - destruct n.
     + reflexivity.
     + erewrite <- IHl1. reflexivity.
+Qed.
+
+Lemma safe_nth_app2 {A : Type} (l1 l2 : list A) (n : nat) (Hn : n >= length l1) H1 H2 :
+  safe_nth (l1 ++ l2) (n ; H1) = safe_nth l2 (n - length l1 ; H2).
+Proof.
+  revert n Hn H1 H2.
+  induction l1; intros.
+  - f_equal. revert H2. rewrite <- minus_n_O.
+    intros. now unify_lt_proofs.
+  - destruct n; simpl.
+    + inversion Hn.
+    + unshelve erewrite IHl1; auto with arith.
 Qed.
 
 Lemma safe_nth_map {A B} (F : A -> B) (l : list A) (n : nat) H1 H2 :
@@ -164,7 +174,7 @@ Proof.
     + apply IHl.
 Qed.
 
-(* One useful lemma about [safe_nth] and [Forall]. *)
+(* A few lemmas about [safe_nth], [Forall], [skipn] and [firstn]. *)
 
 Lemma safe_nth_Forall {A} (P : A -> Prop) (l : list A) (n : nat | n < length l) :
   Forall P l -> P (safe_nth l n).
@@ -175,158 +185,169 @@ Proof.
   - apply safe_nth_In.
 Qed.
 
-
-(** ========== Recursion on a set of variables. ========== *)
-
-Require Import Sorting Orders Permutation.
-
-Lemma Permutation_Forall {A : Type} {P : A -> Prop} {l l' : list A} :
-  Permutation l l' -> Forall P l' -> Forall P l.
+Lemma safe_nth_Foralli_aux {A} (P : nat -> A -> Prop) (l : list A)
+  (i : nat)
+  (n : nat) (Hn : n < length l) :
+  Foralli_aux P i l -> P (i + n) (safe_nth l (n; Hn)).
 Proof.
-  induction 1; intros Htmp;
-  repeat match goal with
-  | H : Forall _ (_ :: _) |- _ => inversion H; subst; clear H
-  end; repeat constructor; auto.
+  intros Hl; revert n Hn.
+  induction Hl; intros [|n'] Hn'; simpl in *.
+  - inversion Hn'.
+  - inversion Hn'.
+  - now rewrite <- plus_n_O.
+  - rewrite <- plus_n_Sm.
+    apply IHHl.
 Qed.
 
-Fixpoint rseq (n : nat) :=
-  match n with
-  | O => []
-  | S n => n :: rseq n
-  end.
-
-Lemma rseq_In (M : nat) (n : nat) : n < M <-> In n (rseq M).
-Proof.
-  induction M; split; intros; simpl in *.
-  - inversion H.
-  - inversion H.
-  - destruct (le_lt_dec M n).
-    + left. omega.
-    + right. now apply IHM.
-  - destruct H.
-    + omega.
-    + constructor. now apply IHM.
-Qed.
-
-Lemma SortedNoDup_seq : forall l, StronglySorted gt l ->
-  forall M, NoDup l -> Forall (fun x => x < M) l ->
-  length l >= M -> l = rseq M.
-Proof.
-  induction 1; intros; simpl in *.
-  - now inv H1.
-  - inv H1; inv H2.
-    specialize (fun H => IHStronglySorted (length l) ltac:(assumption) H (le_n _)).
-    assert (l = rseq (length l)) as Hl.
-    { apply IHStronglySorted.
-      apply Forall_forall; intros.
-      pose proof (Forall_In H0 H1).
-      omega. }
-    assert (~ a < length l) as Ha.
-    { contradict H6. rewrite Hl. now apply rseq_In. }
-    assert (M = S (length l)) as -> by omega.
-    simpl. f_equal.
-    + omega.
-    + assumption.
-Qed.
-
-Lemma SortedNoDup_In : forall l, StronglySorted gt l ->
-  forall M j,
-  NoDup l -> Forall (fun x => x < M) l ->
-  length l >= M -> j < M -> In j l.
+Lemma safe_nth_Foralli {A} (P : nat -> A -> Prop) (l : list A)
+  (n : nat) (Hn : n < length l) :
+  Foralli P l -> P n (safe_nth l (n; Hn)).
 Proof.
   intros.
-  rewrite SortedNoDup_seq with (M := M); try assumption.
-  now apply rseq_In.
+  rewrite <- plus_O_n with (n := n) at 1.
+  now apply safe_nth_Foralli_aux.
 Qed.
 
-Module NatOrder <: TotalLeBool.
-  Definition t := nat.
-  Definition leb x y := Nat.leb y x.
-  Theorem leb_total : forall a1 a2, is_true (leb a1 a2) \/ is_true (leb a2 a1).
+Lemma skipn_length_le {A : Type} (l : list A) {n : nat} :
+  n <= length l -> length (skipn n l) = length l - n.
+Proof.
+  revert n.
+  induction l as [|x l]; intros [|n] **; trivial; simpl.
+  apply IHl. simpl in H. omega.
+Qed.
+
+Lemma skipn_app_1 {A : Type} (n : nat) (l1 l2 : list A) :
+  n <= length l1 -> skipn n (l1 ++ l2) = skipn n l1 ++ l2.
+Proof.
+  revert n.
+  induction l1; intros [|n] **; simpl in *; auto with arith.
+  inv H.
+Qed.
+
+Lemma skipn_app_2 {A : Type} (n : nat) (l1 l2 : list A) :
+  skipn (length l1 + n) (l1 ++ l2) = skipn n l2.
+Proof.
+  now induction l1.
+Qed.
+
+Lemma skipn_skipn {A : Type} (n m : nat) (l : list A) :
+  skipn n (skipn m l) = skipn (n + m) l.
+Proof.
+  revert n m.
+  induction l; intros [|n] [|m]; simpl; auto.
+  - now rewrite <- plus_n_O.
+  - rewrite <- plus_n_Sm.
+    apply IHl.
+Qed.
+
+Lemma skipn_firstn {A : Type} (n m : nat) (l : list A) :
+  skipn n (firstn m l) = firstn (m - n) (skipn n l).
+Proof.
+  revert n m.
+  induction l; intros [|n] [|m]; simpl; auto.
+  now rewrite firstn_nil.
+Qed.
+
+Lemma safe_nth_skipn {A : Type} (n i : nat) (l : list A) (H : i >= n) H1 H2:
+  safe_nth l (i; H1) = safe_nth (skipn n l) (i - n; H2).
+Proof.
+  revert n i H H1 H2.
+  induction l; intros.
+  - inversion H1.
+  - destruct i, n; simpl in *; auto.
+    + inversion H.
+    + now unify_lt_proofs.
+    + erewrite IHl; auto with arith.
+Qed.
+
+Lemma safe_nth_firstn {A : Type} (n i : nat) (l : list A) (H : i < n) H1 H2:
+  safe_nth l (i; H1) = safe_nth (firstn n l) (i; H2).
+Proof.
+  revert n i H H1 H2.
+  induction l; intros.
+  - inversion H1.
+  - destruct i, n; simpl in *; auto.
+    + inversion H.
+    + now unify_lt_proofs.
+    + erewrite IHl; auto with arith.
+Qed.
+
+Lemma safe_nth_trans {A : Type} (n m : nat) (l : list A) (H : n = m) H1 H2:
+  safe_nth l (n; H1) = safe_nth l (m; H2).
+Proof.
+  revert H2. destruct H.
+  intros. simpl in H1. unify_lt_proofs.
+  reflexivity.
+Qed.
+
+(** === Map with the length. *)
+
+Section map_with_length.
+  Context {A B : Type}.
+  Context (f : nat -> A -> B).
+
+  Fixpoint map_with_length (l : list A) : list B :=
+    match l with
+    | [] => []
+    | hd :: tl => f (length l) hd :: map_with_length tl
+    end.
+
+  Lemma map_with_length_length (l : list A) : length (map_with_length l) = length l.
   Proof.
-    unfold leb; intros.
-    destruct (le_lt_dec a1 a2).
-    - right. now apply leb_correct.
-    - left. apply leb_correct. auto with arith.
+    induction l; simpl; auto.
   Qed.
-End NatOrder.
 
-Module Import NatSort := Sort NatOrder.
+  Lemma map_with_length_skipn (l : list A) (i : nat) (Hi : i <= length l) :
+    skipn i (map_with_length l) = map_with_length (skipn i l).
+  Proof.
+    revert i Hi.
+    induction l; intros [|i]; intros; auto.
+    apply IHl. auto with arith.
+  Qed.
 
-Lemma StronglySortedNoDup_ge_gt :
-  forall l,
-  StronglySorted (fun a b => is_true (Nat.leb b a)) l ->
-  NoDup l ->
-  StronglySorted gt l.
+  Lemma safe_nth_map_with_length (l : list A) (n : nat) H1 H2 :
+    safe_nth (map_with_length l) (n; H1) = f (length l - n) (safe_nth l (n; H2)).
+  Proof.
+    revert n H1 H2.
+    induction l; intros [|n] H1 H2; try solve [inversion H1]; auto; simpl.
+    apply IHl.
+  Qed.
+End map_with_length.
+
+Lemma map_with_length_ext {A B : Type} (f g : nat -> A -> B) (H : forall n x, f n x = g n x)
+  (l : list A) :
+  map_with_length f l = map_with_length g l.
 Proof.
-  induction 1; intros.
-  - constructor.
-  - inv H1. specialize (IHStronglySorted H5).
-    constructor.
-    + assumption.
-    + apply Forall_forall; intros.
-      assert (a <> x).
-      { contradict H4; now subst. }
-      apply Forall_In with (2 := H1) in H0; simpl in H0.
-      apply leb_complete in H0. omega.
+  induction l; simpl; auto.
+  f_equal; auto.
 Qed.
 
-(* Main theorem that allows the recursion. *)
-Theorem NoDupFull_In : forall l M j,
-  NoDup l -> Forall (fun x => x < M) l ->
-  length l >= M -> j < M -> In j l.
+Lemma map_map_with_length {A B C : Type} (f : nat -> A -> B) (g : B -> C) (l : list A) :
+  map g (map_with_length f l) = map_with_length (fun n x => g (f n x)) l.
 Proof.
-  intros.
-  pose proof (SortedNoDup_In (sort l)).
-  assert (Permutation (sort l) l).
-  { apply Permutation_sym. apply Permuted_sort. }
-  eapply Permutation_in.
-  { eassumption. }
-  assert (NoDup (sort l)).
-  { eapply Permutation_NoDup'; eassumption. }
-  apply H3 with (M := length l).
-  + assert (StronglySorted (fun a b => is_true (Nat.leb b a)) (sort l)).
-    { apply StronglySorted_sort.
-      unfold Transitive; intros.
-      apply leb_correct. apply leb_complete in H6. apply leb_complete in H7.
-      omega. }
-    now apply StronglySortedNoDup_ge_gt.
-  + assumption.
-  + eapply Permutation_Forall.
-    * eassumption.
-    * eapply Forall_impl with (2 := H0); intros. omega.
-  + erewrite Permutation_length; [|eassumption]. constructor.
-  + omega.
+  induction l; simpl; auto.
+  now rewrite IHl.
 Qed.
 
-(* Induction principle to recurse on a set of variables. *)
-Fixpoint seen_rect' (MAX : nat) (P : list nat -> Type)
-  (f : forall (seen : list nat)
-    (REC : forall (x : nat), x < MAX -> ~ In x seen -> P (x :: seen)), P seen)
-  (fuel : nat) (seen : list nat)
-  (Hseen : NoDup seen /\ Forall (fun x => x < MAX) seen)
-  (Hfuel : MAX <= fuel + length seen)
-    {struct fuel} : P seen.
+Lemma map_with_length_map {A B C : Type} (f : A -> B) (g : B -> C) (l : list A) :
+  map_with_length (fun _ x => g x) (map f l) = map (fun x => g (f x)) l.
 Proof.
-  apply (f seen).
-  intros x Hx HxIn.
-  destruct Hseen as [HseenNoDup HseenMAX].
-  destruct fuel as [|fuel].
-  - exfalso. apply HxIn.
-    apply NoDupFull_In with (M := MAX); assumption.
-  - apply (seen_rect' MAX P f fuel (x :: seen)).
-    repeat split; repeat constructor; try assumption.
-    simpl in *. rewrite <- plus_n_Sm. assumption.
+  induction l; simpl; auto.
+  now rewrite IHl.
 Qed.
 
-Definition seen_rect (MAX : nat) (P : list nat -> Type)
-  (f : forall (seen : list nat)
-    (REC : forall (x : nat), x < MAX -> ~ In x seen -> P (x :: seen)), P seen)
-  (seen : list nat)
-  (Hrec : NoDup seen /\ Forall (fun x => x < MAX) seen) : P seen.
+Lemma map_with_length_map_ext {A B : Type} (f : nat -> A -> B) (g : A -> B)
+  (H : forall n x, f n x = g x) (l : list A) :
+  map_with_length f l = map g l.
 Proof.
-  apply seen_rect' with (MAX := MAX) (fuel := MAX); trivial.
-  apply le_plus_l.
+  induction l; simpl; auto.
+  f_equal; auto.
+Qed.
+
+Lemma map_id {A : Type} (l : list A) :
+  map id l = l.
+Proof.
+  induction l; simpl; f_equal; auto.
 Qed.
 
 (** ========== Regular trees ========== *)
@@ -334,8 +355,8 @@ Qed.
 (* The [crush] tactic is intended to solve most arithmetic goals we will
    encounter. It fails if it cannot solve the goal. *)
 Ltac make_one_simpl :=
-  rewrite map_length in * ||
-  rewrite app_length in * ||
+  autorewrite with rtree in * ||
+  autounfold with rtree in * ||
   match goal with
   | t := _ : _ |- _ => subst t
   | H : _ <=? _ = true |- _ => apply leb_complete in H
@@ -349,7 +370,17 @@ Ltac make_one_simpl :=
   | H : _ ?= _ = Lt |- _ => apply Nat.compare_lt_iff in H
   | H : _ ?= _ = Gt |- _ => apply Nat.compare_gt_iff in H
   end.
-Ltac crush := repeat (try assumption; make_one_simpl; simpl in *); auto; omega.
+Ltac crush := repeat (try eassumption; try make_one_simpl; simpl in *); auto; abstract omega.
+
+Hint Rewrite map_length app_length : rtree.
+Hint Rewrite @skipn_length_le firstn_length_le using crush : rtree.
+Hint Rewrite @map_with_length_length : rtree.
+Hint Rewrite @map_with_length_skipn using crush : rtree.
+
+Ltac reset id :=
+  let id' := constr:(id) in
+  let body := eval unfold id in id' in
+  subst id; set (id := body) in *.
 
 (** Regular trees. *)
 
@@ -381,49 +412,25 @@ Section Rtree.
         end) defs)
     end.
 
-  (** Invariants about this structure. *)
-
-  (* Indices are well-scoped. *)
-  (* Consider [wf_rtree_idx stk tree].
-     The tree [tree] has free variables described by [stk]. *)
-  Inductive wf_rtree_idx : forall (stk : list nat), t -> Prop :=
-  | wfrParam : forall stk i j
-      (Hi : i < length stk) (Hj : j < safe_nth stk (i ; Hi)),
-      wf_rtree_idx stk (rParam i j)
-  | wfrNode : forall stk x sons,
-      Forall (wf_rtree_idx stk) sons ->
-      wf_rtree_idx stk (rNode x sons)
-  | wfrRec : forall stk j defs,
-      j < length defs -> Forall (wf_rtree_idx (length defs :: stk)) defs ->
-      wf_rtree_idx stk (rRec j defs).
-
-  (* Recs are productive. *)
-  (* Consider [wf_rtree_rec ctx defs seen stk tree].
-     The tree [rRec j defs] is closed under [ctx].
-     The tree [tree] has free variables described by [stk ++ [length defs] ++ ctx]. *)
-  Inductive wf_rtree_rec (ctx : list nat) (defs : list t) : forall (seen : list nat) (stk : list nat), t -> Prop :=
-  | wrrParam_nonrec : forall seen stk i j, i <> length stk -> wf_rtree_rec ctx defs seen stk (rParam i j)
-  | wrrParam_rec : forall seen stk i j (Hj : j < length defs),
-      i = length stk -> ~ In j seen ->
-      wf_rtree_rec ctx defs (j :: seen) [] (safe_nth defs (j ; Hj)) ->
-      wf_rtree_rec ctx defs seen stk (rParam i j)
-  | wrrNode : forall seen stk x sons, wf_rtree_rec ctx defs seen stk (rNode x sons)
-  | wrrRec : forall seen stk j loc_defs (Hj : j < length loc_defs),
-      wf_rtree_rec ctx defs seen (length loc_defs :: stk) (safe_nth loc_defs (j ; Hj)) ->
-      wf_rtree_rec ctx defs seen stk (rRec j loc_defs).
-
-  Inductive wf_rtree_rec' : forall (stk : list nat), t -> Prop :=
-  | wrr'Param : forall stk i j, wf_rtree_rec' stk (rParam i j)
-  | wrr'Node : forall stk x sons,
-      Forall (wf_rtree_rec' stk) sons ->
-      wf_rtree_rec' stk (rNode x sons)
-  | wrr'Rec : forall stk j defs,
-      j < length defs -> Forall (wf_rtree_rec' (length defs :: stk)) defs ->
-      Foralli (fun i => wf_rtree_rec stk defs [i] []) defs ->
-      wf_rtree_rec' stk (rRec j defs).
-
-  Definition wf_rtree (stk : list nat) (tree : t) : Prop :=
-    wf_rtree_idx stk tree /\ wf_rtree_rec' stk tree.
+  Fixpoint t_ind'' (P : t -> Prop)
+    (fParam : forall i j, P (rParam i j))
+    (fNode : forall x sons, Forall P sons ->  P (rNode x sons))
+    (fRec : forall j defs, Forall P defs -> P (rRec j defs))
+      (tree : t) : P tree :=
+    let REC := t_ind'' P fParam fNode fRec in
+    match tree with
+    | rParam i j => fParam i j
+    | rNode x sons => fNode x sons ((fix aux l : Forall _ l :=
+        match l with
+        | [] => Forall_nil _
+        | hd :: tl => Forall_cons hd (REC hd) (aux tl)
+        end) sons)
+    | rRec j defs => fRec j defs ((fix aux l : Forall _ l :=
+        match l with
+        | [] => Forall_nil _
+        | hd :: tl => Forall_cons hd (REC hd) (aux tl)
+        end) defs)
+    end.
 
   (** Lifting and substitution. *)
   Definition lift_rtree_rec_body (F : nat -> nat -> t -> t)
@@ -438,358 +445,669 @@ Section Rtree.
     lift_rtree_rec_body lift_rtree_rec depth n tree.
   Definition lift_rtree n tree := (lift_rtree_rec 0 n tree).
 
-  (* Lifting preserves scoping of indices. *)
-  Lemma wf_lift_rtree_idx :
-    forall ctx newstk (newd := length newstk) tree stk (d := length stk),
-      wf_rtree_idx (stk ++ ctx) tree ->
-      wf_rtree_idx ((stk ++ newstk) ++ ctx) (lift_rtree_rec d newd tree).
-  Proof.
-    intros ctx newstk newd tree stk.
-    induction stk, tree using t_ind'; intros d Hidx;
-    inv Hidx; simpl in *.
-    - destruct (Nat.leb_spec d i); econstructor.
-      + destruct (Nat.le_exists_sub d i ltac:(crush)) as [i' [-> _]].
-        assert (i' < length ctx) as Hi' by (clear Hj; crush).
-        gen_safe_proof.
-        replace (i' + d + newd) with (length (stk ++ newstk) + i') by crush.
-        intros. erewrite safe_nth_app2.
-        subst d. erewrite safe_nth_app2' in Hj.
-        eassumption.
-      + gen_safe_proof.
-        rewrite app_assoc_reverse.
-        intros. erewrite safe_nth_app1.
-        erewrite safe_nth_app1 in Hj.
-        eassumption.
-    - constructor. apply Forall_map.
-      apply Forall_Impl with (1 := H2) (2 := H).
-    - constructor.
-      + crush.
-      + apply Forall_map. rewrite map_length.
-        apply Forall_Impl with (1 := H4) (2 := H).
-    Unshelve. all: try crush. clear Hj; crush.
-  Qed.
-
-  (* Lifting preserves the productivity of a particular Rec node. *)
-  Lemma wf_lift_rtree_rec :
-    forall defs (ddefs := length defs) seen,
-    NoDup seen /\ Forall (fun x => x < length defs) seen ->
-    forall ctx stk' (d' := length stk'),
-    Forall (wf_rtree_idx (ddefs :: stk' ++ ctx)) defs ->
-    forall newstk (newd := length newstk),
-    forall tree stk (d := length stk),
-    wf_rtree_idx (stk ++ ddefs :: stk' ++ ctx) tree ->
-    wf_rtree_rec (stk' ++ ctx) defs seen stk tree ->
-    let F := lift_rtree_rec (d + S d') newd in
-    let F' := lift_rtree_rec (S d') newd in
-      wf_rtree_rec ((stk' ++ newstk) ++ ctx) (map F' defs) seen stk (F tree).
-  Proof.
-    intros defs ddefs seen Hrec ctk stk' d' Hidx_defs newstk newd.
-    pattern seen. refine (seen_rect ddefs _ _ seen Hrec); clear seen Hrec;
-    intros seen REC. intros tree stk.
-    induction stk, tree using t_ind';
-    intros d Hidx_tree Hwf_tree F F';
-    inv Hidx_tree; inv Hwf_tree; unfold F; simpl in *.
-    - destruct (Nat.leb_spec (d + S d') i).
-      + constructor. crush.
-      + constructor. crush.
-    - assert (d + S d' <=? length stk = false) as -> by crush.
-      econstructor 2; trivial.
-      erewrite safe_nth_map.
-      apply REC; try eassumption.
-      apply Forall_In with (1 := Hidx_defs).
-      apply safe_nth_In.
-    - constructor.
-    - rename defs0 into locdefs.
-      econstructor.
-      erewrite safe_nth_map.
-      eapply Forall_forall' in H.
-      + rewrite map_length. apply H; try eassumption.
-        apply Forall_In with (1 := H4). apply safe_nth_In.
-      + apply safe_nth_In.
-    Unshelve. all: crush.
-  Qed.
-
-  (* Lifting preserves the productivity of Rec nodes. *)
-  Lemma wf_lift_rtree_rec' :
-    forall ctx newstk (newd := length newstk) tree stk (d := length stk),
-      wf_rtree_idx (stk ++ ctx) tree ->
-      wf_rtree_rec' (stk ++ ctx) tree ->
-      wf_rtree_rec' ((stk ++ newstk) ++ ctx) (lift_rtree_rec d newd tree).
-  Proof.
-    intros ctx newstk newd tree stk.
-    induction stk, tree using t_ind'; intros d Hidx Hwf;
-    inv Hidx; inv Hwf; simpl in *.
-    - destruct (Nat.leb_spec d i); constructor.
-    - constructor. apply Forall_map.
-      apply Forall_forall; intros.
-      apply Forall_forall' with (2 := H0) in H.
-      apply Forall_forall' with (2 := H0) in H2.
-      apply Forall_forall' with (2 := H0) in H3.
-      auto.
-    - constructor.
-      + now rewrite map_length.
-      + rewrite map_length. apply Forall_map.
-        apply Forall_forall; intros.
-        apply Forall_forall with (2 := H0) in H.
-        apply Forall_forall with (2 := H0) in H4.
-        apply Forall_forall with (2 := H0) in H6.
-        auto.
-      + apply Foralli_map.
-        apply Foralli_impl with (2 := H7); intros.
-        apply wf_lift_rtree_rec; trivial.
-        * repeat split; repeat constructor; crush.
-        * apply Forall_In with (1 := H4). assumption.
-  Qed.
-
-  Theorem wf_lift_rtree :
-    forall ctx newstk (newd := length newstk) tree stk (d := length stk),
-    wf_rtree (stk ++ ctx) tree ->
-    wf_rtree ((stk ++ newstk) ++ ctx) (lift_rtree_rec d newd tree).
-  Proof.
-    intros ctx newstk newd tree stk d [Hidx Hwf].
-    split.
-    - now apply wf_lift_rtree_idx.
-    - now apply wf_lift_rtree_rec'.
-  Qed.
-
-  (* A tree that has been lifted above a Rec is productive for this Rec, since
-     it does not have any free variable referring to this Rec. *)
-  Lemma wf_rtree_rec_deep :
-    forall defs (ddefs := length defs) seen ctx stk' (d' := length stk')
-      stk'' (d'' := length stk''),
-    Forall (wf_rtree_idx (ddefs :: stk' ++ ctx)) defs ->
-    forall tree stk (d := length stk),
-    wf_rtree_idx (stk ++ ctx) tree ->
-    wf_rtree_rec (stk' ++ ctx) defs seen (stk ++ stk'') (lift_rtree_rec d (d'' + S d') tree).
-  Proof.
-    intros defs ddefs seen ctx stk' d' stk'' d'' Hidx_defs.
-    intros tree stk.
-    induction stk, tree using t_ind'; intros d Hidx;
-    inv Hidx; unfold lift_rtree; simpl in *.
-    - destruct (Nat.leb_spec d i); constructor; crush.
-    - constructor.
-    - rename defs0 into locdefs.
-      econstructor. erewrite safe_nth_map.
-      gen_safe_proof. rewrite map_length.
-      intros. eapply Forall_forall' in H.
-      + apply H. eapply Forall_In.
-        * eassumption.
-        * apply safe_nth_In.
-      + apply safe_nth_In.
-    Unshelve. all: crush.
-  Qed.
-
   Definition subst_rtree_rec_body (F : nat -> list t -> t -> t)
-    (depth : nat) (sub : list t) (tree : t) : t :=
-    match tree with
-    | rParam i j =>
-      match nat_compare depth i with
-      | Eq => lift_rtree depth (rRec j sub)
-      | Gt => rParam i j
-      | Lt => rParam (pred i) j
-      end
-    | rNode x sons => rNode x (List.map (F depth sub) sons)
-    | rRec j defs => rRec j (List.map (F (S depth) sub) defs)
-    end.
+  (depth : nat) (sub : list t) (tree : t) : t :=
+  match tree with
+  | rParam i j =>
+    match nat_compare depth i with
+    | Eq => lift_rtree depth (rRec j sub)
+    | Gt => rParam i j
+    | Lt => rParam (pred i) j
+    end
+  | rNode x sons => rNode x (List.map (F depth sub) sons)
+  | rRec j defs => rRec j (List.map (F (S depth) sub) defs)
+  end.
 
   Fixpoint subst_rtree_rec (depth : nat) (sub : list t) (tree : t) {struct tree} : t :=
     subst_rtree_rec_body subst_rtree_rec depth sub tree.
   Definition subst_rtree sub tree := (subst_rtree_rec 0 sub tree).
 
-  (* Substitution preserves scoping of indices. *)
-  Lemma wf_subst_rtree_idx :
-    forall ctx sub (dsub := length sub),
-    Forall (wf_rtree_idx (dsub :: ctx)) sub ->
-    forall tree stk (d := length stk),
-      wf_rtree_idx (stk ++ dsub :: ctx) tree ->
-      wf_rtree_idx (stk ++ ctx) (subst_rtree_rec d sub tree).
+  (* A few permutation lemmas. *)
+  Lemma lift0 :
+    forall tree k,
+    lift_rtree_rec k 0 tree = tree.
   Proof.
-    intros ctx sub dsub Hidx_sub tree stk.
-    induction stk, tree using t_ind'; intros d Hidx;
-    inv Hidx; simpl in *.
-    - destruct (Nat.compare_spec d i).
-      + subst. subst d.
-        constructor; rewrite map_length.
-        * pose proof (safe_nth_app2' stk (dsub :: ctx) O).
-          simpl in H. erewrite H in Hj; clear H; crush.
-        * fold lift_rtree_rec. apply Forall_map.
-          apply Forall_impl with (2 := Hidx_sub); intros.
-          apply wf_lift_rtree_idx with (stk := [dsub]).
+    induction tree using t_ind''; intros; simpl in *;
+    only 2-3: (f_equal; rewrite <- map_id;
+      apply map_ext_in; intros tree HtreeIn; apply (Forall_In H HtreeIn)).
+    destruct (Nat.leb_spec k i); f_equal; crush.
+  Qed.
+
+  Lemma simpl_lift :
+    forall tree i p k n,
+    i <= k + n ->
+    k <= i ->
+    lift_rtree_rec i p (lift_rtree_rec k n tree) = lift_rtree_rec k (p + n) tree.
+  Proof.
+    induction tree using t_ind''; intros; simpl in *;
+    only 2-3: (f_equal; rewrite !map_map; apply map_ext_in; intros tree HtreeIn).
+    - repeat (try (f_equal; crush);
+      match goal with
+      | |- context [if ?a <=? ?b then _ else _] => destruct (Nat.leb_spec a b)
+      | |- context [match ?a ?= ?b with _ => _ end] => destruct (Nat.compare_spec a b)
+      end; subst; simpl; unfold subst_rtree, lift_rtree).
+    - apply (Forall_In H HtreeIn); crush.
+    - apply (Forall_In H HtreeIn); crush.
+  Qed.
+
+  Lemma commut_lift_subst :
+    forall tree sub k n p,
+    k <= p ->
+    lift_rtree_rec k n (subst_rtree_rec p sub tree) =
+    subst_rtree_rec (n + p) sub (lift_rtree_rec k n tree).
+  Proof.
+    induction tree using t_ind''; intros; simpl in *;
+    only 2-3: (f_equal; rewrite !map_map; apply map_ext_in; intros tree HtreeIn).
+    - repeat (try (f_equal; crush);
+      match goal with
+      | |- context [if ?a <=? ?b then _ else _] => destruct (Nat.leb_spec a b)
+      | |- context [match ?a ?= ?b with _ => _ end] => destruct (Nat.compare_spec a b)
+      end; subst; simpl; unfold subst_rtree, lift_rtree).
+      f_equal; rewrite map_map; apply map_ext; intros tree.
+      apply simpl_lift; crush.
+    - apply (Forall_In H HtreeIn); crush.
+    - rewrite plus_n_Sm. apply (Forall_In H HtreeIn); crush.
+  Qed.
+
+  Lemma simpl_subst :
+    forall tree sub n k p,
+    p <= n + k ->
+    k <= p ->
+    subst_rtree_rec p sub (lift_rtree_rec k (S n) tree) =
+    lift_rtree_rec k n tree.
+  Proof.
+    induction tree using t_ind''; intros; simpl in *;
+    only 2-3: (f_equal; rewrite !map_map; apply map_ext_in; intros tree HtreeIn).
+    - repeat (try (f_equal; crush);
+      match goal with
+      | |- context [if ?a <=? ?b then _ else _] => destruct (Nat.leb_spec a b)
+      | |- context [match ?a ?= ?b with _ => _ end] => destruct (Nat.compare_spec a b)
+      end; subst; simpl; unfold subst_rtree, lift_rtree).
+    - apply (Forall_In H HtreeIn); crush.
+    - apply (Forall_In H HtreeIn); crush.
+  Qed.
+
+  Lemma distr_subst :
+    forall tree P N p n,
+    subst_rtree_rec (p + n) P (subst_rtree_rec p N tree) =
+    subst_rtree_rec p (map (subst_rtree_rec (S n) P) N) (subst_rtree_rec (S (p + n)) P tree).
+  Proof.
+    induction tree using t_ind''; intros; simpl in *;
+    only 2-3: (f_equal; rewrite !map_map; apply map_ext_in; intros tree HtreeIn).
+    - destruct (Nat.compare_spec p i); subst; simpl.
+      + destruct i; subst.
+        * simpl; unfold lift_rtree; simpl.
+          f_equal; rewrite !map_map; apply map_ext; intros tree.
+          rewrite commut_lift_subst; crush.
+        * assert (S i + n ?= i = Gt) as -> by crush.
+          simpl. assert (i ?= i = Eq) as -> by crush.
+          unfold lift_rtree; simpl.
+          f_equal; rewrite !map_map; apply map_ext; intros tree.
+          rewrite commut_lift_subst; f_equal; crush.
+      + destruct (Nat.compare_spec (p + n) (pred i)).
+        * destruct i; try crush.
+          assert (p + n ?= i = Eq) as -> by crush.
+          unfold lift_rtree; simpl.
+          f_equal; rewrite !map_map; apply map_ext; intros tree.
+          rewrite simpl_subst; crush.
+        * destruct i; try crush.
+          assert (p + n ?= i = Lt) as -> by crush.
+          simpl. assert (p ?= i = Lt) as -> by crush.
+          crush.
+        * destruct i; try crush.
+          assert (p + n ?= i = Gt) as -> by crush.
+          simpl. assert (p ?= S i = Lt) as -> by crush.
+          crush.
+      + assert (p + n ?= i = Gt) as -> by crush.
+        destruct i.
+        * simpl. assert (p ?= 0 = Gt) as -> by crush.
+          crush.
+        * assert (p + n ?= i = Gt) as -> by crush.
+          simpl. assert (p ?= S i = Gt) as -> by crush.
+          crush.
+    - apply (Forall_In H HtreeIn).
+    - apply (Forall_In H HtreeIn _ _ (S p)).
+  Qed.
+
+  (** Invariants about this structure. *)
+
+  (* We will consider any tree under a context made of a list of free variables,
+     and then a list of definitions and seen variables. *)
+  Definition Context : Set := list nat.
+  Definition Stack : Set := list (list t * list nat).
+
+  (* We can convert a Stack to a Context simply by forgetting every information
+     except the number of mutally recursive definitions. *)
+  Definition Context_of_Stack : Stack -> Context := map (fun '(x, _) => length x).
+  Hint Unfold Context_of_Stack : rtree.
+
+  Definition map_Stack (f : nat -> t -> t) : Stack -> Stack :=
+    map_with_length (fun m '(defs, seen) =>
+      (map (f m) defs, seen)).
+  Hint Unfold map_Stack : rtree.
+
+  Lemma map_Stack_seen :
+    forall f stk i (Hi : i < length stk) (Hi' : i < length (map_Stack f stk)),
+      snd (safe_nth (map_Stack f stk) (i; Hi')) = snd (safe_nth stk (i; Hi)).
+  Proof.
+    intros.
+    unfold map_Stack.
+    rewrite safe_nth_map_with_length with (H2 := Hi).
+    destruct safe_nth. reflexivity.
+  Qed.
+
+  Lemma map_Stack_safe_nth f g stk i (Hi : i < length stk) (Hi' : i < length (map_Stack f stk)) :
+      (forall x, g x = f (length stk - i) x) ->
+      fst (safe_nth (map_Stack f stk) (i; Hi')) = map g (fst (safe_nth stk (i; Hi))).
+  Proof.
+    intros.
+    unfold map_Stack.
+    rewrite safe_nth_map_with_length with (H2 := Hi).
+    destruct safe_nth.
+    now apply map_ext.
+  Qed.
+
+  Lemma Context_of_map_Stack f stk :
+    Context_of_Stack (map_Stack f stk) = Context_of_Stack stk.
+  Proof.
+    unfold Context_of_Stack, map_Stack.
+    rewrite map_map_with_length.
+    apply map_with_length_map_ext.
+    intros n0 [defs seen].
+    now rewrite map_length.
+  Qed.
+
+  Lemma lt_in_Ctx {ctx : Context} {stk : Stack} {i} (Hi : i < length stk + length ctx)
+    (Hi' : length stk <= i) : i - length stk < length ctx.
+  Proof. omega. Qed.
+
+  Inductive wf_rtree : forall (ctx : Context) (stk : Stack), t -> Prop :=
+  | wfParam_free : forall ctx stk i j (Hi : i < length stk + length ctx)
+      (Hi' : length stk <= i) (Hj : j < safe_nth ctx (i - length stk; lt_in_Ctx Hi Hi')),
+      wf_rtree ctx stk (rParam i j)
+  | wfParam_rec : forall ctx stk i j (Hi : i < length stk),
+      let defs_seen := safe_nth stk (i; Hi) in
+      let defs := fst defs_seen in
+      let seen := snd defs_seen in
+      let stk' := skipn (S i) stk in
+      forall (Hj : j < length defs),
+      ~ In j seen ->
+      wf_rtree ctx ((defs, j :: seen) :: stk') (safe_nth defs (j; Hj)) ->
+      wf_rtree ctx stk (rParam i j)
+  | wfNode : forall ctx stk x sons,
+      Forall (wf_rtree (Context_of_Stack stk ++ ctx) []) sons ->
+      wf_rtree ctx stk (rNode x sons)
+  | wfRec : forall ctx stk defs,
+      (Foralli (fun j => wf_rtree ctx ((defs, [j]) :: stk)) defs) ->
+      forall j (Hj : j < length defs),
+      wf_rtree ctx stk (rRec j defs).
+
+  Definition wf_rtree_ind' (P : Context -> Stack -> t -> Prop)
+    (fwfParam_free :
+      forall (ctx : list nat) (stk : list (list t * list nat))
+        (i j : nat) (Hi : i < length stk + length ctx) (Hi' : length stk <= i),
+        j < safe_nth ctx (i - length stk; lt_in_Ctx Hi Hi') ->
+        P ctx stk (rParam i j))
+    (fwfParam_rec :
+      forall (ctx : Context) (stk : list (list t * list nat))
+        (i j : nat) (Hi : i < length stk),
+        let defs_seen := safe_nth stk (i; Hi) in
+        let defs := fst defs_seen in
+        let seen := snd defs_seen in
+        let stk' := skipn (S i) stk in
+        forall Hj : j < length defs,
+        ~ In j seen ->
+        wf_rtree ctx ((defs, j :: seen) :: stk') (safe_nth defs (j; Hj)) ->
+        P ctx ((defs, j :: seen) :: stk') (safe_nth defs (j; Hj)) ->
+        P ctx stk (rParam i j))
+    (fwfNode :
+      forall (ctx : list nat) (stk : Stack) (x : X) (sons : list t),
+        Forall (wf_rtree (Context_of_Stack stk ++ ctx) []) sons ->
+        Forall (P (Context_of_Stack stk ++ ctx) []) sons ->
+        P ctx stk (rNode x sons))
+    (fwfRec :
+      forall (ctx : Context) (stk : list (list t * list nat))
+        (defs : list t),
+        Foralli (fun j => wf_rtree ctx ((defs, [j]) :: stk)) defs ->
+        Foralli (fun j => P ctx ((defs, [j]) :: stk)) defs ->
+        forall j (Hj : j < length defs),
+        P ctx stk (rRec j defs)) :
+    forall (ctx : Context) (stk : Stack) (tree : t) (Hwf : wf_rtree ctx stk tree),
+      P ctx stk tree :=
+  fix F ctx stk tree Hwf : P ctx stk tree :=
+  match Hwf with
+  | wfParam_free ctx stk i j Hi Hi' Hj =>
+      fwfParam_free ctx stk i j Hi Hi' Hj
+  | wfParam_rec ctx stk i j Hi _ defs seen stk' Hj HjNotIn Hwf =>
+      fwfParam_rec ctx stk i j Hi Hj HjNotIn Hwf
+        (F ctx ((defs, j :: seen) :: stk') (safe_nth defs (j; Hj)) Hwf)
+  | wfNode ctx stk x sons Hwf =>
+      fwfNode ctx stk x sons Hwf (Forall_ind
+        (fun sons => _ sons)
+        (Forall_nil _)
+        (fun _ _ Htree _ Hrec => Forall_cons _ (F _ _ _ Htree) Hrec) Hwf)
+  | wfRec ctx stk defs Hdefs j Hj =>
+      fwfRec ctx stk defs Hdefs (Foralli_aux_ind _ _
+    (fun n defs' => Foralli_aux (fun j => P ctx ((defs, [j]) :: stk)) n defs')
+    (fun n => Foralli_nil _ _)
+    (fun _ _ _ Htree _ Hrec => Foralli_cons _ _ _ _ (F _ _ _ Htree) Hrec)
+    0 defs Hdefs) j Hj
+  end.
+
+  Lemma wf_weaken :
+    forall ctx stk tree,
+    wf_rtree ctx stk tree ->
+    forall n (Hn : n <= length stk),
+    wf_rtree (Context_of_Stack (skipn n stk) ++ ctx) (firstn n stk) tree.
+  Proof.
+    induction 1 using wf_rtree_ind'; intros.
+    - econstructor.
+      erewrite safe_nth_app2; only 2: crush.
+      erewrite safe_nth_trans.
+      + eassumption.
+      + crush.
+    - destruct (le_lt_dec (n) i).
+      + econstructor 1.
+        erewrite safe_nth_app1.
+        unfold Context_of_Stack.
+        erewrite safe_nth_map.
+        gen_safe_proof.
+        rewrite firstn_length_le; only 2: crush.
+        intros. erewrite <- safe_nth_skipn; only 2: crush.
+        gen_safe_proof; intros; unify_lt_proofs.
+        destruct safe_nth.
+        assumption.
+      + econstructor 2.
+        * erewrite <- safe_nth_firstn; only 2: crush.
+          gen_safe_proof; intros; unify_lt_proofs.
           assumption.
+        * repeat gen_safe_proof.
+          intros Hs.
+          erewrite <- safe_nth_firstn; only 2: crush.
+          gen_safe_proof; intros; unify_lt_proofs.
+          intros; unify_lt_proofs.
+          reset defs_seen; reset defs; reset seen.
+          specialize (IHwf_rtree (n - i) ltac:(crush)).
+          subst stk'.
+          replace (skipn n stk)
+             with (skipn (n - i) ((defs, j :: seen) :: skipn (S i) stk));
+          swap 1 2.
+          { rewrite <- Nat.succ_pred_pos with (n := n - i); only 2: crush.
+            simpl. rewrite skipn_skipn. f_equal. crush. }
+          replace ((defs, j :: seen) :: skipn (S i) (firstn n stk))
+             with (firstn (n - i) ((defs, j :: seen) :: skipn (S i) stk));
+          swap 1 2.
+          { rewrite <- Nat.succ_pred_pos with (n := n - i); only 2: crush.
+            simpl. f_equal. replace (pred (n - i)) with (n - S i) by crush.
+            now rewrite skipn_firstn. }
+          assumption.
+    - constructor.
+      unfold Context_of_Stack.
+      rewrite app_assoc.
+      rewrite <- map_app.
+      rewrite firstn_skipn.
+      assumption.
+    - constructor; only 2: crush.
+      apply Foralli_impl with (2 := H0).
+      intros i tree Hi HtreeIn Hwf.
+      specialize (Hwf (S n) ltac:(crush)).
+      assumption.
+  Unshelve.
+    all: try crush.
+      gen_safe_proof; intros.
+      erewrite <- safe_nth_firstn; only 2: crush.
+      eassumption.
+  Qed.
+
+  Definition lift_Stack (d n : nat) : Stack -> Stack :=
+    map_Stack (fun m def => lift_rtree_rec (m + d) n def).
+  Hint Unfold lift_Stack : rtree.
+
+  Lemma lift_Stack_seen :
+    forall d n stk i (Hi : i < length stk) (Hi' : i < length (lift_Stack d n stk)),
+      snd (safe_nth (lift_Stack d n stk) (i; Hi')) = snd (safe_nth stk (i; Hi)).
+  Proof.
+    intros. apply map_Stack_seen.
+  Qed.
+
+  Lemma lift_Stack_safe_nth (d : nat) (n : nat) (stk : Stack)
+    (i : nat) (Hi : i < length stk) (Hi' : i < length (lift_Stack d n stk)) :
+    let hd := safe_nth (lift_Stack d n stk) (i; Hi') in
+    let stk' := skipn (S i) (lift_Stack d n stk) in
+    let F := lift_rtree_rec (length (hd :: stk') + d) n in
+      fst hd = map F (fst (safe_nth stk (i; Hi))).
+  Proof.
+    apply map_Stack_safe_nth.
+    intros.
+    f_equal. crush.
+  Qed.
+
+  Lemma Context_of_lift_Stack (d : nat) (n : nat) (stk : Stack) :
+    Context_of_Stack (lift_Stack d n stk) = Context_of_Stack stk.
+  Proof.
+    apply Context_of_map_Stack.
+  Qed.
+
+  Lemma wf_lift_rtree :
+    forall newctx ctx stk tree,
+      wf_rtree ctx stk tree ->
+      forall n (Hn : n <= length ctx),
+      let F := lift_rtree_rec (length stk + n) (length newctx) in
+      let FS := lift_Stack n (length newctx) in
+      wf_rtree (firstn n ctx ++ newctx ++ skipn n ctx) (FS stk) (F tree).
+  Proof.
+    induction 1 using wf_rtree_ind'; intros; subst F; simpl.
+    - destruct (Nat.leb_spec (length stk + n) i).
       + econstructor.
-        destruct (Nat.le_exists_sub d (pred i) ltac:(crush)) as [i' [Hi' _]].
-        assert (i = i' + S d) by crush.
-        gen_safe_proof. rewrite Hi'; clear Hi'; subst i.
-        intros. subst d. erewrite safe_nth_app2'.
-        revert Hi Hj.
-        replace (stk ++ dsub :: ctx) with ((stk ++ [dsub]) ++ ctx)
-        by (repeat rewrite app_assoc_reverse; reflexivity).
-        replace (i' + S (length stk)) with (i' + length (stk ++ [dsub]))
-        by crush.
-        intros. erewrite safe_nth_app2' in Hj.
-        eassumption.
+        erewrite safe_nth_app2; only 2: crush.
+        erewrite safe_nth_app2; only 2: crush.
+        erewrite safe_nth_skipn with (n0 := n) in H; only 2: crush.
+        erewrite safe_nth_trans.
+        * eassumption.
+        * clear H; crush.
       + econstructor.
         erewrite safe_nth_app1.
-        erewrite safe_nth_app1 in Hj.
-        eassumption.
+        erewrite safe_nth_firstn with (n0 := n) in H; only 2: crush.
+        erewrite safe_nth_trans.
+        * eassumption.
+        * clear; crush.
+    - assert (length stk + n <=? i = false) as -> by crush.
+      econstructor 2.
+      + unfold FS. erewrite lift_Stack_seen. eassumption.
+      + specialize (IHwf_rtree n Hn).
+        simpl in IHwf_rtree. unfold FS.
+        erewrite lift_Stack_seen.
+        gen_safe_proof. gen_safe_proof.
+        erewrite lift_Stack_safe_nth.
+        gen_safe_proof. intros Hp.
+        change (length
+           (safe_nth (lift_Stack n (length newctx) stk) (i; Hp)
+            :: skipn (S i) (lift_Stack n (length newctx) stk)) + n) with
+            (S (length (skipn (S i) (lift_Stack n (length newctx) stk))) + n).
+        clear Hp.
+        gen_safe_proof; intros. unify_lt_proofs.
+        intros Hp. erewrite safe_nth_map. clear Hp.
+        crush.
     - constructor. apply Forall_map.
-      apply Forall_Impl with (1 := H2) (2 := H).
-    - constructor.
-      + crush.
-      + apply Forall_map. rewrite map_length.
-        apply Forall_Impl with (1 := H4) (2 := H).
+      apply Forall_Impl with (1 := H0).
+      apply Forall_forall. intros tree HtreeIn.
+      apply Forall_forall' with (x0 := tree) in H0; trivial.
+      intros.
+      specialize (H0 (length (Context_of_Stack stk) + n) ltac:(crush)).
+      simpl in H0.
+      unfold Context_of_Stack in H0 at 1 3 5.
+      subst FS.
+      rewrite Context_of_lift_Stack.
+      replace (length stk) with (length (Context_of_Stack stk)) in H0 at 1 2 by crush.
+      repeat rewrite firstn_app_2 in H0.
+      rewrite skipn_app_2 in H0.
+      rewrite app_assoc_reverse in H0.
+      crush.
+    - econstructor; only 2: crush.
+      apply Foralli_map.
+      apply Foralli_impl with (2 := H0); clear H0.
+      intros i tree Hi HtreeIn Hwf.
+      specialize (Hwf n Hn). simpl in *.
+      assumption.
     Unshelve.
-      clear Hj; crush.
-      clear Hi; crush.
-      all: crush.
+      all: try crush.
+      subst FS. erewrite lift_Stack_safe_nth. crush.
   Qed.
 
-  Lemma wf_subst_rtree_rec :
-    forall defs (ddefs := length defs) seen,
-    NoDup seen /\ Forall (fun x => x < length defs) seen ->
-    forall ctx sub (dsub := length sub),
-    Forall (wf_rtree_idx (dsub :: ctx)) sub ->
-    forall stk' (d' := length stk'),
-    Forall (wf_rtree_idx (ddefs :: stk' ++ dsub :: ctx)) defs ->
-    forall tree stk (d := length stk),
-    wf_rtree_idx (stk ++ ddefs :: stk' ++ dsub :: ctx) tree ->
-    wf_rtree_rec (stk' ++ dsub :: ctx) defs seen stk tree ->
-    let F := subst_rtree_rec (d + S d') sub in
-    let F' := subst_rtree_rec (S d') sub in
-      wf_rtree_rec (stk' ++ ctx) (map F' defs) seen stk (F tree).
+  Lemma wf_lift_rtree_deep :
+    forall newstk ctx stk tree,
+    wf_rtree ctx stk tree ->
+    let FS := lift_Stack 0 (length newstk) in
+    let F := lift_rtree_rec (length stk) (length newstk) in
+    wf_rtree ctx (FS stk ++ newstk) (F tree).
   Proof.
-    intros defs ddefs seen Hrec ctx sub dsub Hidx_sub stk' d' Hidx_defs.
-    pattern seen. refine (seen_rect ddefs _ _ seen Hrec); clear seen Hrec;
-    intros seen REC. intros tree stk.
-    induction stk, tree using t_ind';
-    intros d Hidx Hwf F F';
-    inv Hidx; inv Hwf; unfold F; simpl in *.
-    - destruct (Nat.compare_spec (d + S d') i).
-      + apply wf_rtree_rec_deep with (stk := []).
-        * apply Forall_map. apply Forall_impl with (2 := Hidx_defs).
-          intros. rewrite map_length.
-          apply wf_subst_rtree_idx with (stk := ddefs :: stk'); assumption.
-        * constructor; trivial.
-          subst i. revert Hi Hj.
-          replace (d + S d') with (length (stk ++ ddefs :: stk') + 0) by crush.
-          replace (stk ++ ddefs :: stk' ++ dsub :: ctx)
-          with ((stk ++ ddefs :: stk') ++ dsub :: ctx)
-          by (repeat rewrite app_assoc_reverse; reflexivity).
-          intros. erewrite safe_nth_app2 in Hj.
-          assumption.
-      + constructor. crush.
-      + constructor. assumption.
-    - assert (d + S d' ?= length stk = Gt) as -> by crush.
-      econstructor 2; trivial.
-      erewrite safe_nth_map.
-      apply REC; try eassumption.
-      apply Forall_In with (1 := Hidx_defs).
-      apply safe_nth_In.
-    - constructor.
-    - rename defs0 into locdefs.
+    induction 1 using wf_rtree_ind'; intros; subst F; simpl in *.
+    - assert (length stk <=? i = true) as -> by crush.
       econstructor.
-      erewrite safe_nth_map.
-      eapply Forall_forall' in H.
-      + rewrite map_length. apply H; try eassumption.
-        apply Forall_In with (1 := H4). apply safe_nth_In.
-      + apply safe_nth_In.
-    Unshelve. all: crush.
-  Qed.
-
-  (* Substitution preserves the productivity of Rec nodes. *)
-  Lemma wf_subst_rtree_rec' :
-    forall ctx sub (dsub := length sub),
-      Forall (wf_rtree_idx (dsub :: ctx)) sub ->
-      Forall (wf_rtree_rec' (dsub :: ctx)) sub ->
-      Foralli (fun i => wf_rtree_rec ctx sub [i] []) sub ->
-      forall tree stk (d := length stk),
-      wf_rtree_idx (stk ++ dsub :: ctx) tree ->
-      wf_rtree_rec' (stk ++ dsub :: ctx) tree ->
-      wf_rtree_rec' (stk ++ ctx) (subst_rtree_rec d sub tree).
-  Proof.
-    intros ctx sub dsub Hidx_sub Hwf_sub Hwfi_sub tree stk.
-    induction stk, tree using t_ind'; intros d Hidx Hwf;
-    inv Hidx; inv Hwf; simpl in *.
-    - destruct (Nat.compare_spec d i); constructor; fold lift_rtree_rec.
-      + rewrite map_length. subst i.
-        subst d. erewrite safe_nth_app2' with (n := O) (l1 := stk) in Hj.
-        assumption.
-      + apply Forall_map. apply Forall_forall; intros.
-        apply Forall_forall' with (2 := H0) in Hidx_sub.
-        apply Forall_forall' with (2 := H0) in Hwf_sub.
-        rewrite map_length.
-        apply wf_lift_rtree_rec' with (stk := [dsub]); assumption.
-      + apply Foralli_map. apply Foralli_impl with (2 := Hwfi_sub); intros.
-        apply wf_lift_rtree_rec with (stk' := []); trivial.
-        * repeat split; repeat constructor; crush.
-        * apply Forall_In with (1 := Hidx_sub). assumption.
+      erewrite safe_nth_trans.
+      + eassumption.
+      + crush.
+    - assert (length stk <=? i = false) as -> by crush.
+      econstructor 2.
+      + erewrite safe_nth_app1. subst FS.
+        erewrite lift_Stack_seen. eassumption.
+      + gen_safe_proof. erewrite safe_nth_app1.
+        subst FS. erewrite lift_Stack_safe_nth.
+        intros.
+        erewrite safe_nth_map.
+        gen_safe_proof. gen_safe_proof.
+        gen_safe_proof.
+        intros ?; unify_lt_proofs.
+        intros ?; unify_lt_proofs.
+        intros Hs'.
+        erewrite lift_Stack_seen.
+        gen_safe_proof; intros; unify_lt_proofs.
+        reset defs_seen; reset defs; reset seen; reset stk'.
+        simpl.
+        replace (length (skipn (S i) (lift_Stack 0 (length newstk) stk)))
+        with (length stk') by crush.
+        replace (skipn (S i) (lift_Stack 0 (length newstk) stk ++ newstk))
+        with (lift_Stack 0 (length newstk) stk' ++ newstk); swap 1 2.
+        { rewrite skipn_app_1; only 2: crush.
+          unfold lift_Stack, map_Stack.
+          rewrite map_with_length_skipn; crush. }
+        rewrite <- plus_n_O at 2. apply IHwf_rtree.
     - constructor. apply Forall_map.
-      apply Forall_forall; intros.
-      apply Forall_forall' with (2 := H0) in H.
-      apply Forall_forall' with (2 := H0) in H2.
-      apply Forall_forall' with (2 := H0) in H3.
-      auto.
-    - constructor.
-      + now rewrite map_length.
-      + rewrite map_length. apply Forall_map.
-        apply Forall_forall; intros.
-        apply Forall_forall with (2 := H0) in H.
-        apply Forall_forall with (2 := H0) in H4.
-        apply Forall_forall with (2 := H0) in H6.
-        auto.
-      + apply Foralli_map.
-        apply Foralli_impl with (2 := H7); intros.
-        apply wf_subst_rtree_rec; trivial.
-        * repeat split; repeat constructor; crush.
-        * apply Forall_In with (1 := H4). assumption.
-    Unshelve. all: crush.
+      apply Forall_impl with (2 := H).
+      intros tree Htree.
+      replace (Context_of_Stack (FS stk ++ newstk) ++ ctx) with
+              (Context_of_Stack stk ++ Context_of_Stack newstk ++ ctx); swap 1 2.
+      { subst FS. rewrite app_assoc. f_equal.
+        unfold Context_of_Stack. rewrite map_app.
+        f_equal. rewrite Context_of_lift_Stack. reflexivity. }
+      replace (Context_of_Stack stk) with
+              (firstn (length stk) (Context_of_Stack stk ++ ctx)); swap 1 2.
+      { rewrite firstn_app.
+        assert (length stk - length (Context_of_Stack stk) = 0) as -> by crush.
+        rewrite firstn_O. rewrite app_nil_r.
+        rewrite firstn_all2; crush. }
+      replace (ctx) with
+              (skipn (length stk) (Context_of_Stack stk ++ ctx)) at 2; swap 1 2.
+      { replace (length stk) with (length (Context_of_Stack stk) + 0) by crush.
+        now rewrite skipn_app_2. }
+      replace (length newstk) with (length (Context_of_Stack newstk)) by crush.
+      apply wf_lift_rtree with (stk := []); crush.
+    - econstructor; only 2: crush.
+      apply Foralli_map.
+      apply Foralli_impl with (2 := H0); clear H0.
+      intros i tree Hi HtreeIn Hwf.
+      rewrite plus_n_O with (n := length stk) at 1.
+      assumption.
+    Unshelve.
+      all: try crush.
+      erewrite safe_nth_app1. subst FS. erewrite lift_Stack_safe_nth. crush.
+    Unshelve.
+      all: try crush.
   Qed.
 
-  Theorem wf_subst_rtree :
-    forall ctx sub (dsub := length sub),
-    Forall (wf_rtree_idx (dsub :: ctx)) sub ->
-    Forall (wf_rtree_rec' (dsub :: ctx)) sub ->
-    Foralli (fun i => wf_rtree_rec ctx sub [i] []) sub ->
-    forall tree stk (d := length stk),
-    wf_rtree (stk ++ dsub :: ctx) tree ->
-    wf_rtree (stk ++ ctx) (subst_rtree_rec d sub tree).
+  Definition subst_Stack (d : nat) (sub : list t) : Stack -> Stack :=
+    map_Stack (fun m def => subst_rtree_rec (m + d) sub def).
+  Hint Unfold subst_Stack : rtree.
+
+  Lemma subst_Stack_seen :
+    forall d sub stk i (Hi : i < length stk) (Hi' : i < length (subst_Stack d sub stk)),
+      snd (safe_nth (subst_Stack d sub stk) (i; Hi')) = snd (safe_nth stk (i; Hi)).
   Proof.
-    intros ctx sub dsub Hidx_sub Hwf_sub Hwfi_sub tree stk d [Hidx Hwf].
-    split.
-    - now apply wf_subst_rtree_idx.
-    - now apply wf_subst_rtree_rec'.
+    intros.
+    apply map_Stack_seen.
   Qed.
 
-  (* Alternative formulation. *)
+  Lemma subst_Stack_safe_nth d sub stk i (Hi : i < length stk) (Hi' : i < length (subst_Stack d sub stk)) :
+    let hd := safe_nth (subst_Stack d sub stk) (i; Hi') in
+    let stk' := skipn (S i) (subst_Stack d sub stk) in
+    let F := subst_rtree_rec (length (hd :: stk') + d) sub in
+      fst hd = map F (fst (safe_nth stk (i; Hi))).
+  Proof.
+    apply map_Stack_safe_nth.
+    intros. f_equal. crush.
+  Qed.
+
+  Lemma Context_of_subst_Stack (d : nat) (sub : list t) (stk : Stack) :
+    Context_of_Stack (subst_Stack d sub stk) = Context_of_Stack stk.
+  Proof.
+    apply Context_of_map_Stack.
+  Qed.
+
+  Lemma wf_subst_rtree :
+    forall sub (ctx : Context) (stk : Stack) (tree : t),
+      wf_rtree ctx stk tree ->
+      forall n (Hn : n < length ctx)
+      (Hsub : Foralli (fun j => wf_rtree (skipn (S n) ctx) [(sub, [j])]) sub)
+      (Hnsub : safe_nth ctx (n; Hn) = length sub),
+      let F := subst_rtree_rec (length stk + n) sub in
+      let FS := subst_Stack n sub in
+      wf_rtree (firstn n ctx ++ skipn (S n) ctx) (FS stk) (F tree).
+  Proof.
+    induction 1 using wf_rtree_ind'; intros; subst F; simpl.
+    - destruct (Nat.compare_spec (length stk + n) i).
+      + subst.
+        unfold lift_rtree.
+        revert H. gen_safe_proof.
+        rewrite minus_plus. intros; unify_lt_proofs.
+        intros.
+        rewrite <- simpl_lift with (i := 0); try crush.
+        replace (length stk) with (length (FS stk)) by crush.
+        apply wf_lift_rtree_deep with (stk := []).
+        replace n with (length (firstn n ctx)) at 3 by crush.
+        apply wf_lift_rtree with (newctx := firstn n ctx) (ctx := skipn (S n) ctx)
+          (stk := []) (n := 0); only 2: crush.
+        econstructor; crush.
+      + econstructor.
+        erewrite safe_nth_app2; only 2: crush.
+        erewrite safe_nth_skipn with (n0 := S n) in H; only 2: crush.
+        erewrite safe_nth_trans.
+        * eassumption.
+        * clear H. crush.
+      + econstructor.
+        erewrite safe_nth_app1.
+        erewrite safe_nth_firstn with (n0 := n) in H; only 2: crush.
+        erewrite safe_nth_trans.
+        * eassumption.
+        * clear; crush.
+    - assert (length stk + n ?= i = Gt) as -> by crush.
+      econstructor 2.
+      + unfold FS. erewrite subst_Stack_seen. eassumption.
+      + specialize (IHwf_rtree n Hn Hsub Hnsub).
+        simpl in IHwf_rtree. unfold FS.
+        erewrite subst_Stack_seen.
+        gen_safe_proof. gen_safe_proof.
+        erewrite subst_Stack_safe_nth.
+        gen_safe_proof. intros Hp.
+        change (length
+           (safe_nth (subst_Stack n sub stk) (i; Hp)
+            :: skipn (S i) (subst_Stack n sub stk)) + n) with
+            (S (length (skipn (S i) (subst_Stack n sub stk))) + n).
+        clear Hp.
+        gen_safe_proof; intros; unify_lt_proofs.
+        intros Hp. erewrite safe_nth_map. clear Hp.
+        crush.
+    - constructor. apply Forall_map.
+      apply Forall_Impl with (1 := H).
+      apply Forall_forall. intros tree HtreeIn.
+      apply Forall_forall' with (x0 := tree) in H0; trivial.
+      intros. simpl in H0.
+      subst FS. rewrite Context_of_subst_Stack.
+      rewrite app_assoc.
+      rewrite <- firstn_app_2.
+      rewrite <- skipn_app_2 with (l1 := Context_of_Stack stk).
+      unfold Context_of_Stack at 1 3. rewrite map_length.
+      rewrite <- plus_n_Sm.
+      unshelve eapply H0.
+      + crush.
+      + intros. rewrite plus_n_Sm.
+        replace (length stk) with (length (Context_of_Stack stk)) by crush.
+        rewrite skipn_app_2. auto.
+      + gen_safe_proof.
+        replace (length stk) with (length (Context_of_Stack stk)) by crush.
+        intros.
+        erewrite safe_nth_app2; only 2: crush.
+        gen_safe_proof.
+        rewrite minus_plus.
+        intros; unify_lt_proofs.
+        assumption.
+    - econstructor; only 2: crush.
+      apply Foralli_map.
+      apply Foralli_impl with (2 := H0); clear H0.
+      intros i tree Hi HtreeIn Hwf.
+      specialize (Hwf n Hn). simpl in *.
+      apply Hwf; assumption.
+  Unshelve.
+    all: try crush.
+    subst FS. erewrite subst_Stack_safe_nth. crush.
+  Qed.
+
+(* Not needed?
+  Lemma wf_subst_rtree_deep :
+    forall sub ctx stk tree,
+    wf_rtree ctx stk tree ->
+    forall n (Hn : n < length stk)
+    (Hsub : Foralli (fun j => wf_rtree (Context_of_Stack (skipn (S n) stk) ++ ctx)
+      ((sub, [j]) :: stk)) sub)
+    (Hnsub : fst (safe_nth stk (n; Hn)) = sub),
+    let F := subst_rtree_rec n sub in
+    let FS := subst_Stack 0 sub in
+    wf_rtree ctx (FS (firstn n stk) ++ skipn (S n) stk) (F tree).
+  Proof.
+    induction 1 using wf_rtree_ind'; intros; subst F; simpl in *.
+  Admitted.
+*)
+
   Corollary wf_subst_rtree' :
-    forall ctx sub (dsub := length sub) j,
-      wf_rtree ctx (rRec j sub) ->
-    forall tree stk (d := length stk),
-    wf_rtree (stk ++ dsub :: ctx) tree ->
-    wf_rtree (stk ++ ctx) (subst_rtree_rec d sub tree).
+    forall ctx sub (dsub := length sub)
+    (Hsub : Foralli (fun j => wf_rtree ctx [(sub, [j])]) sub)
+    tree stk (d := length stk),
+    wf_rtree (stk ++ dsub :: ctx) [] tree ->
+    wf_rtree (stk ++ ctx) [] (subst_rtree_rec d sub tree).
   Proof.
-    intros ctx sub dsub j [Hidx_rec Hwf_rec].
-    inv Hidx_rec; inv Hwf_rec.
-    now apply wf_subst_rtree.
+    intros ctx sub dsub Hsub.
+    intros.
+    pose proof (wf_subst_rtree).
+    specialize (H0 sub (stk ++ dsub :: ctx) [] tree H d).
+    simpl in H0.
+    replace (stk ++ ctx) with (firstn d (stk ++ dsub :: ctx) ++
+      skipn (S d) (stk ++ dsub :: ctx)); swap 1 2.
+    { f_equal.
+      - rewrite firstn_app.
+        subst d. rewrite Nat.sub_diag.
+        rewrite firstn_all. simpl.
+        apply app_nil_r.
+      - change (dsub :: ctx) with ([dsub] ++ ctx).
+        rewrite app_assoc. rewrite plus_n_O with (n := S d).
+        replace (S d) with (length (stk ++ [dsub])) by crush.
+        apply skipn_app_2. }
+    eapply H0.
+    - intros.
+      change (dsub :: ctx) with ([dsub] ++ ctx).
+      rewrite app_assoc. rewrite plus_n_O with (n := S d).
+      replace (S d) with (length (stk ++ [dsub])) by crush.
+      rewrite skipn_app_2. now apply Hsub.
+    - erewrite safe_nth_app2; only 2: crush.
+      subst d.
+      gen_safe_proof. rewrite Nat.sub_diag.
+      intros. reflexivity.
+  Unshelve.
+    all: crush.
   Qed.
 
   (* Even more specialized. *)
   Corollary wf_subst_rtree'' :
-    forall ctx sub (dsub := length sub) j,
-      wf_rtree ctx (rRec j sub) ->
-    forall (Hj : j < dsub),
+    forall ctx sub (dsub := length sub) j (Hj : j < dsub),
+      wf_rtree ctx [] (rRec j sub) ->
       let tree := subst_rtree sub (safe_nth sub (j; Hj)) in
-      wf_rtree ctx tree.
+      wf_rtree ctx [] tree.
   Proof.
-    intros ctx sub dsub j Hwf Hj tree.
-    apply wf_subst_rtree' with (j := j) (stk := []).
-    - assumption.
-    - destruct Hwf as [Hidx Hwf]; inv Hidx; inv Hwf.
-      split.
-      + apply Forall_In with (1 := H3).
-        apply safe_nth_In.
-      + apply Forall_In with (1 := H5).
-        apply safe_nth_In.
+    intros ctx sub dsub j Hj Hsub tree.
+    apply wf_subst_rtree' with (stk := []).
+    - now inv Hsub.
+    - simpl.
+      apply wf_weaken with (ctx := ctx) (stk := [(sub, [j])]) (n := 0); only 2: crush.
+      inv Hsub.
+      now apply safe_nth_Foralli.
   Qed.
 
   (* === Expansion === *)
@@ -801,46 +1119,107 @@ Section Rtree.
       (forall (Hj : j < length defs), rtree_bar (subst_rtree defs (safe_nth defs (j; Hj)))) ->
       rtree_bar (rRec j defs).
 
-  Program Fixpoint expand_rec (tree : t)
-    (tree_wf : exists ctx, wf_rtree ctx tree) (bar : rtree_bar tree) {struct bar} : t :=
-    match tree with
-    | rRec j defs =>
+  Program Fixpoint expand_rec (tree : t) (Hwf : exists ctx, wf_rtree ctx [] tree)
+    (bar : rtree_bar tree) {struct bar} : t :=
+      match tree with
+      | rRec j defs =>
         let Hj : j < length defs := _ in
         let def := safe_nth defs (j; Hj) in
         let tree' := subst_rtree defs def in
           expand_rec tree' _ _
-    | t => t
-    end.
+      | t => t
+      end.
 
-  (* Providing [Hj]. *)
   Next Obligation.
-    destruct H as [Hidx _].
-    inv Hidx.
-    assumption.
+    now inv H.
   Defined.
 
-  (* Proving the recursive argument is well-formed. *)
   Next Obligation.
-    rename tree_wf into ctx.
-    exists ctx. apply wf_subst_rtree''.
-    assumption.
+    rename Hwf into ctx.
+    exists ctx.
+    now apply wf_subst_rtree''.
   Defined.
 
-  (* Providing a termination certificate for the recursive argument. *)
   Next Obligation.
     simpl.
     inv bar.
     apply H1.
   Defined.
 
-  Definition expand (tree : t) (tree_wf : exists ctx, wf_rtree ctx tree) : t.
+  Fixpoint wf_expand_rec (tree : t) (ctx : Context)
+    (Hwf : wf_rtree ctx [] tree)
+    (bar : rtree_bar tree) {struct bar} :
+    wf_rtree ctx [] (expand_rec tree (ex_intro _ ctx Hwf) bar).
+  Proof.
+    destruct bar; try assumption.
+    apply wf_expand_rec with (tree := subst_rtree _ _).
+  Qed.
+
+  Theorem wf_bar (ctx : Context) (stk : Stack) (tree : t) :
+    wf_rtree ctx stk tree ->
+      let tree' := fold_left (fun tree '(defs, seen) => subst_rtree defs tree) stk tree in
+      rtree_bar tree'.
+  Proof.
+    induction 1 using wf_rtree_ind'; simpl in *.
+    - revert dependent i.
+      induction stk as [|[defs seen] stk']; intros; simpl.
+      + constructor.
+      + unfold subst_rtree; simpl.
+        destruct i; only 1: (crush).
+        apply (IHstk' i ltac:(crush) ltac:(crush)).
+        erewrite safe_nth_trans.
+        * eassumption.
+        * crush.
+    - revert dependent i.
+      induction stk as [|[defs' seen'] stk]; intros; simpl in *.
+      + constructor.
+      + unfold subst_rtree; simpl.
+        destruct i.
+        * clear IHstk.
+          unfold skipn in stk'; subst stk' defs_seen defs seen; simpl in *.
+          unfold lift_rtree. rewrite lift0.
+          clear H0 Hi H.
+          revert dependent defs'.
+          induction stk as [|[defs seen] stk']; intros; simpl in *.
+          -- constructor. intros; unify_lt_proofs. assumption.
+          -- eapply IHstk'; clear IHstk'.
+             erewrite safe_nth_map.
+             gen_safe_proof; intros; unify_lt_proofs.
+             unfold subst_rtree.
+             rewrite <- distr_subst.
+             apply IHwf_rtree.
+        * eapply IHstk; eauto.
+    - clear H H0. revert sons.
+      induction stk as [|[defs seen] stk']; intros; simpl; try constructor.
+      apply IHstk'.
+    - clear H. revert dependent defs.
+      induction stk as [|[defs' seen] stk']; intros; simpl in *.
+      + constructor. intros; unify_lt_proofs.
+        now apply safe_nth_Foralli.
+      + unfold subst_rtree; simpl.
+        eapply IHstk'; only 2: crush; clear IHstk'.
+        apply Foralli_map.
+        apply Foralli_impl with (2 := H0); clear H0.
+        intros i tree Hi HtreeIn Hwf.
+        unfold subst_rtree.
+        rewrite <- distr_subst.
+        apply Hwf.
+  Unshelve.
+    all: crush.
+  Qed.
+
+  Definition expand (tree : t) (tree_wf : exists ctx, wf_rtree ctx [] tree) : t.
   Proof.
     refine (expand_rec tree tree_wf _).
-    destruct tree; constructor.
-    intros.
+    destruct tree_wf as [ctx Hwf].
+    apply wf_bar with (ctx := ctx) (stk := []).
+    assumption.
   Defined.
 
-  (* TODO Try to define an equivalent [expand'] which maintains a stack of
-     explicit substitutions, and use it to derive the termination certificate? *)
+  Theorem wf_expand (tree : t) (ctx : Context) (Hwf : wf_rtree ctx [] tree) :
+    wf_rtree ctx [] (expand tree (ex_intro _ ctx Hwf)).
+  Proof.
+    apply wf_expand_rec.
+  Qed.
 
 End Rtree.
